test/test_runner_generated.cljs
@@ -188,6 +188,7 @@
             [hyperopen.state.trading.identity-and-submit-policy-test]
             [hyperopen.state.trading.market-summary-test]
             [hyperopen.state.trading.order-form-key-policy-test]
+            [hyperopen.state.trading.order-form-ownership-formal-conformance-test]
             [hyperopen.state.trading.order-form-state-test]
             [hyperopen.state.trading.order-request-test]
             [hyperopen.state.trading.submit-policy-formal-conformance-test]
@@ -612,6 +613,7 @@
              'hyperopen.state.trading.identity-and-submit-policy-test
              'hyperopen.state.trading.market-summary-test
              'hyperopen.state.trading.order-form-key-policy-test
+             'hyperopen.state.trading.order-form-ownership-formal-conformance-test
              'hyperopen.state.trading.order-form-state-test
              'hyperopen.state.trading.order-request-test
              'hyperopen.state.trading.submit-policy-formal-conformance-test
